add deleted flag

LeanYjs/Item.lean
@@ -36,18 +36,18 @@ inductive YjsPtr : Type where
   deriving Repr, DecidableEq
 
 inductive YjsItem : Type where
-| item (origin : YjsPtr) (rightOrigin : YjsPtr) : YjsId -> A -> YjsItem
+| item (origin : YjsPtr) (rightOrigin : YjsPtr) (id : YjsId) (content : A) (deleted : Bool) : YjsItem
 deriving Repr, DecidableEq
 end
 
 def YjsItem.origin {A : Type} : YjsItem A -> YjsPtr A
-  | YjsItem.item origin _ _ _ => origin
+  | YjsItem.item origin _ _ _ _ => origin
 
 def YjsItem.rightOrigin {A : Type} : YjsItem A -> YjsPtr A
-  | YjsItem.item _ rightOrigin _ _ => rightOrigin
+  | YjsItem.item _ rightOrigin _ _ _ => rightOrigin
 
 def YjsItem.content {A : Type} : YjsItem A -> A
-  | YjsItem.item _ _ _ content => content
+  | YjsItem.item _ _ _ content _ => content
 
 mutual
 def YjsPtr.size {A : Type} : YjsPtr A -> Nat
@@ -56,7 +56,7 @@ def YjsPtr.size {A : Type} : YjsPtr A -> Nat
   | YjsPtr.last => 0
 
 def YjsItem.size {A : Type} : YjsItem A -> Nat
-  | YjsItem.item origin rightOrigin _ _ =>
+  | YjsItem.item origin rightOrigin _ _ _ =>
     origin.size + rightOrigin.size + 2
 end
 
@@ -80,4 +80,4 @@ instance : Coe (YjsItem A) (YjsPtr A) where
   coe item := YjsPtr.itemPtr item
 
 def YjsItem.id {A : Type} : YjsItem A -> YjsId
-| YjsItem.item _ _ id _ => id
+| YjsItem.item _ _ id _ _ => id
